compiler/src/ExprImp.v
@@ -1,128 +1,121 @@
-Require Import Coq.Lists.List.
-Import ListNotations.
+Require Import Coq.Lists.List. Import ListNotations.
+Require Import Coq.Program.Tactics.
+Require Import bbv.DepEqNat.
 Require Import lib.LibTacticsMin.
 Require Import riscv.util.BitWidths.
+Require Import riscv.Utility.
+Require Export bedrock2.Syntax.
+Require Export bedrock2.Semantics.
+Require Import bedrock2.Macros.
 Require Import compiler.util.Common.
 Require Import compiler.util.Tactics.
 Require Import compiler.Op.
 Require Import compiler.StateCalculus.
-Require Import bbv.DepEqNat.
 Require Import compiler.NameWithEq.
-Require Import Coq.Program.Tactics.
 Require Import compiler.Memory.
-Require Import riscv.Utility.
 
 
 Section ExprImp1.
 
-  Context {mword: Set}.
-  Context {MW: MachineWidth mword}.
+  Context {p : unique! Semantics.parameters}.
 
-  Context {Name: NameWithEq}.
-  Notation var := (@name Name).
-  Existing Instance eq_name_dec.
-  Context {FName : NameWithEq}.
-  Notation func := (@name FName).
+  Notation mword := (@Semantics.word p).
+  Context {MW: MachineWidth mword}.  
+  
+  Notation var := (@varname (@syntax p)).
+  Notation func := (@funname (@syntax p)).
 
   Context {stateMap: MapFunctions var (mword)}.
-  Notation state := (map var (mword)).
+  Notation state := (map var mword).
   Context {varset: SetFunctions var}.
   Notation vars := (set var).
 
-  Ltac state_calc := state_calc_generic (@name Name) (mword).
-  Ltac set_solver := set_solver_generic (@name Name).
-
-  Inductive expr: Set :=
-    | ELit(v: Z): expr
-    | EVar(x: var): expr
-    | EOp(op: binop)(e1 e2: expr): expr.
-
-  Inductive stmt: Set :=
-    | SLoad(x: var)(addr: expr): stmt
-    | SStore(addr val: expr): stmt
-    | SSet(x: var)(e: expr): stmt
-    | SIf(cond: expr)(bThen bElse: stmt): stmt
-    | SWhile(cond: expr)(body: stmt): stmt
-    | SSeq(s1 s2: stmt): stmt
-    | SSkip: stmt
-    | SCall(binds: list var)(f: func)(args: list expr).
+  Hypothesis actname_empty: actname = Empty_set.
+  
+  Ltac state_calc := state_calc_generic (@varname (@syntax p)) (@Semantics.word p).
+  Ltac set_solver := set_solver_generic (@varname (@syntax p)).
 
   Fixpoint eval_expr(st: state)(e: expr): option mword :=
     match e with
-    | ELit v => Return (ZToReg v)
-    | EVar x => get st x
-    | EOp op e1 e2 =>
+    | expr.literal v => Return (ZToReg v)
+    | expr.var x => get st x
+    | expr.load x a => None (* TODO *)
+    | expr.op op e1 e2 =>
         v1 <- eval_expr st e1;
         v2 <- eval_expr st e2;
-        Return (eval_binop op v1 v2)
+        Return (interp_binop op v1 v2)
     end.
 
   Section WithEnv.
-    Context {funcMap: MapFunctions func (list var * list var * stmt)}.
-    Notation env := (map func (list var * list var * stmt)).
+    Context {funcMap: MapFunctions func (list var * list var * cmd)}.
+    Notation env := (map func (list var * list var * cmd)).
     Context (e: env).
 
-    Fixpoint eval_stmt(f: nat)(st: state)(m: mem)(s: stmt): option (state * mem) :=
+    Fixpoint eval_cmd(f: nat)(st: state)(m: mem)(s: cmd): option (state * mem) :=
       match f with
       | 0 => None (* out of fuel *)
       | S f => match s with
+        (* TODO
         | SLoad x a =>
             a <- eval_expr st a;
             v <- read_mem a m;
             Return (put st x v, m)
-        | SStore a v =>
+        *)
+        | cmd.store number_of_bytes_IGNORED_TODO a v =>
             a <- eval_expr st a;
             v <- eval_expr st v;
             m <- write_mem a v m;
             Return (st, m)
-        | SSet x e =>
+        | cmd.set x e =>
             v <- eval_expr st e;
             Return (put st x v, m)
-        | SIf cond bThen bElse =>
+        | cmd.cond cond bThen bElse =>
             v <- eval_expr st cond;
-            eval_stmt f st m (if reg_eqb v (ZToReg 0) then bElse else bThen)
-        | SWhile cond body =>
+            eval_cmd f st m (if reg_eqb v (ZToReg 0) then bElse else bThen)
+        | cmd.while cond body =>
             v <- eval_expr st cond;
             if reg_eqb v (ZToReg 0) then Return (st, m) else
-              p <- eval_stmt f st m body;
+              p <- eval_cmd f st m body;
               let '(st, m) := p in
-              eval_stmt f st m (SWhile cond body)
-        | SSeq s1 s2 =>
-            p <- eval_stmt f st m s1;
+              eval_cmd f st m (cmd.while cond body)
+        | cmd.seq s1 s2 =>
+            p <- eval_cmd f st m s1;
             let '(st, m) := p in
-            eval_stmt f st m s2
-        | SSkip => Return (st, m)
-        | SCall binds fname args =>
+            eval_cmd f st m s2
+        | cmd.skip => Return (st, m)
+        | cmd.call binds fname args =>
           fimpl <- get e fname;
           let '(params, rets, fbody) := fimpl in
           argvs <- option_all (List.map (eval_expr st) args);
           st0 <- putmany params argvs empty_map;
-          st1m' <- eval_stmt f st0 m fbody;
+          st1m' <- eval_cmd f st0 m fbody;
           let '(st1, m') := st1m' in
           retvs <- option_all (List.map (get st1) rets);
           st' <- putmany binds retvs st;
           Return (st', m')
+        | cmd.interact _ _ _ => None (* unsupported *)
         end
       end.
 
     Fixpoint expr_size(e: expr): nat :=
       match e with
-      | ELit _ => 8
-      | EVar _ => 1
-      | EOp op e1 e2 => S (S (expr_size e1 + expr_size e2))
+      | expr.literal _ => 8
+      | expr.load _ e => S (expr_size e)
+      | expr.var _ => 1
+      | expr.op op e1 e2 => S (S (expr_size e1 + expr_size e2))
       end.
 
-    Fixpoint stmt_size(s: stmt): nat :=
+    Fixpoint cmd_size(s: cmd): nat :=
       match s with
-      | SLoad x a => S (expr_size a)
-      | SStore a v => S (expr_size a + expr_size v)
-      | SSet x e => S (expr_size e)
-      | SIf cond bThen bElse => S (expr_size cond + stmt_size bThen + stmt_size bElse)
-      | SWhile cond body => S (expr_size cond + stmt_size body)
-      | SSeq s1 s2 => S (stmt_size s1 + stmt_size s2)
-      | SSkip => 1
-      | SCall binds f args =>
+      | cmd.store _ a v => S (expr_size a + expr_size v)
+      | cmd.set x e => S (expr_size e)
+      | cmd.cond cond bThen bElse => S (expr_size cond + cmd_size bThen + cmd_size bElse)
+      | cmd.while cond body => S (expr_size cond + cmd_size body)
+      | cmd.seq s1 s2 => S (cmd_size s1 + cmd_size s2)
+      | cmd.skip => 1
+      | cmd.call binds f args =>
           S (length binds + length args + List.fold_right Nat.add O (List.map expr_size args))
+      | cmd.interact _ _ _ => 1
       end.
 
     Local Ltac inversion_lemma :=
@@ -136,183 +129,187 @@ Section ExprImp1.
       inversionss;
       eauto 16.
 
-    Lemma invert_eval_SLoad: forall fuel initialSt initialM x e final,
-      eval_stmt (S fuel) initialSt initialM (SLoad x e) = Some final ->
-      exists a v, eval_expr initialSt e = Some a /\
-                  read_mem a initialM = Some v /\
-                  final = (put initialSt x v, initialM).
-    Proof. inversion_lemma. Qed.
-
-    Lemma invert_eval_SStore: forall fuel initialSt initialM a v final,
-      eval_stmt (S fuel) initialSt initialM (SStore a v) = Some final ->
+    Lemma invert_eval_store: forall fuel initialSt initialM a v final nbytes,
+      eval_cmd (S fuel) initialSt initialM (cmd.store nbytes a v) = Some final ->
       exists av vv finalM, eval_expr initialSt a = Some av /\
                            eval_expr initialSt v = Some vv /\
                            write_mem av vv initialM = Some finalM /\
                            final = (initialSt, finalM).
     Proof. inversion_lemma. Qed.
 
-    Lemma invert_eval_SSet: forall f st1 m1 p2 x e,
-      eval_stmt (S f) st1 m1 (SSet x e) = Some p2 ->
+    Lemma invert_eval_set: forall f st1 m1 p2 x e,
+      eval_cmd (S f) st1 m1 (cmd.set x e) = Some p2 ->
       exists v, eval_expr st1 e = Some v /\ p2 = (put st1 x v, m1).
     Proof. inversion_lemma. Qed.
 
-    Lemma invert_eval_SIf: forall f st1 m1 p2 cond bThen bElse,
-      eval_stmt (S f) st1 m1 (SIf cond bThen bElse) = Some p2 ->
+    Lemma invert_eval_cond: forall f st1 m1 p2 cond bThen bElse,
+      eval_cmd (S f) st1 m1 (cmd.cond cond bThen bElse) = Some p2 ->
       exists cv,
         eval_expr st1 cond = Some cv /\ 
-        (cv <> ZToReg 0 /\ eval_stmt f st1 m1 bThen = Some p2 \/
-         cv = ZToReg 0  /\ eval_stmt f st1 m1 bElse = Some p2).
+        (cv <> ZToReg 0 /\ eval_cmd f st1 m1 bThen = Some p2 \/
+         cv = ZToReg 0  /\ eval_cmd f st1 m1 bElse = Some p2).
     Proof. inversion_lemma. Qed.
 
-    Lemma invert_eval_SWhile: forall st1 m1 p3 f cond body,
-      eval_stmt (S f) st1 m1 (SWhile cond body) = Some p3 ->
+    Lemma invert_eval_while: forall st1 m1 p3 f cond body,
+      eval_cmd (S f) st1 m1 (cmd.while cond body) = Some p3 ->
       exists cv,
         eval_expr st1 cond = Some cv /\
-        (cv <> ZToReg 0 /\ (exists st2 m2, eval_stmt f st1 m1 body = Some (st2, m2) /\ 
-                                     eval_stmt f st2 m2 (SWhile cond body) = Some p3) \/
+        (cv <> ZToReg 0 /\ (exists st2 m2, eval_cmd f st1 m1 body = Some (st2, m2) /\ 
+                                     eval_cmd f st2 m2 (cmd.while cond body) = Some p3) \/
          cv = ZToReg 0 /\ p3 = (st1, m1)).
     Proof. inversion_lemma. Qed.
 
-    Lemma invert_eval_SSeq: forall st1 m1 p3 f s1 s2,
-      eval_stmt (S f) st1 m1 (SSeq s1 s2) = Some p3 ->
-      exists st2 m2, eval_stmt f st1 m1 s1 = Some (st2, m2) /\ eval_stmt f st2 m2 s2 = Some p3.
+    Lemma invert_eval_seq: forall st1 m1 p3 f s1 s2,
+      eval_cmd (S f) st1 m1 (cmd.seq s1 s2) = Some p3 ->
+      exists st2 m2, eval_cmd f st1 m1 s1 = Some (st2, m2) /\ eval_cmd f st2 m2 s2 = Some p3.
     Proof. inversion_lemma. Qed.
 
-    Lemma invert_eval_SSkip: forall st1 m1 p2 f,
-      eval_stmt (S f) st1 m1 SSkip = Some p2 ->
+    Lemma invert_eval_skip: forall st1 m1 p2 f,
+      eval_cmd (S f) st1 m1 cmd.skip = Some p2 ->
       p2 = (st1, m1).
     Proof. inversion_lemma. Qed.
 
-    Lemma invert_eval_SCall : forall st m1 p2 f binds fname args,
-      eval_stmt (S f) st m1 (SCall binds fname args) = Some p2 ->
+    Lemma invert_eval_call : forall st m1 p2 f binds fname args,
+      eval_cmd (S f) st m1 (cmd.call binds fname args) = Some p2 ->
       exists params rets fbody argvs st0 st1 m' retvs st',
         get e fname = Some (params, rets, fbody) /\
         option_all (List.map (eval_expr st) args) = Some argvs /\
         putmany params argvs empty_map = Some st0 /\
-        eval_stmt f st0 m1 fbody = Some (st1, m') /\
+        eval_cmd f st0 m1 fbody = Some (st1, m') /\
         option_all (List.map (get st1) rets) = Some retvs /\
         putmany binds retvs st = Some st' /\
         p2 = (st', m').
     Proof. inversion_lemma. Qed.
+
+    Lemma invert_eval_interact : forall st m1 p2 f binds fname args,
+      eval_cmd (S f) st m1 (cmd.interact binds fname args) = Some p2 ->
+      False.
+    Proof. inversion_lemma. Qed.
+
   End WithEnv.
 
   (* Returns a list to make it obvious that it's a finite set. *)
   Fixpoint allVars_expr(e: expr): list var :=
     match e with
-    | ELit v => []
-    | EVar x => [x]
-    | EOp op e1 e2 => (allVars_expr e1) ++ (allVars_expr e2)
+    | expr.literal v => []
+    | expr.var x => [x]
+    | expr.load nbytes e => allVars_expr e
+    | expr.op op e1 e2 => (allVars_expr e1) ++ (allVars_expr e2)
     end.
 
-  Fixpoint allVars_stmt(s: stmt): list var := 
+  Fixpoint allVars_cmd(s: cmd): list var := 
     match s with
-    | SLoad v e => v :: allVars_expr e
-    | SStore a e => (allVars_expr a) ++ (allVars_expr e)
-    | SSet v e => v :: allVars_expr e
-    | SIf c s1 s2 => (allVars_expr c) ++ (allVars_stmt s1) ++ (allVars_stmt s2)
-    | SWhile c body => (allVars_expr c) ++ (allVars_stmt body)
-    | SSeq s1 s2 => (allVars_stmt s1) ++ (allVars_stmt s2)
-    | SSkip => []
-    | SCall binds _ args => binds ++ List.fold_right (@List.app _) nil (List.map allVars_expr args)
+    | cmd.store _ a e => (allVars_expr a) ++ (allVars_expr e)
+    | cmd.set v e => v :: allVars_expr e
+    | cmd.cond c s1 s2 => (allVars_expr c) ++ (allVars_cmd s1) ++ (allVars_cmd s2)
+    | cmd.while c body => (allVars_expr c) ++ (allVars_cmd body)
+    | cmd.seq s1 s2 => (allVars_cmd s1) ++ (allVars_cmd s2)
+    | cmd.skip => []
+    | cmd.call binds _ args => binds ++ List.fold_right (@List.app _) nil (List.map allVars_expr args)
+    | cmd.interact _ _ _ => [] (* TODO *)
     end.
 
   (* Returns a static approximation of the set of modified vars.
      The returned set might be too big, but is guaranteed to include all modified vars. *)
-  Fixpoint modVars(s: stmt): vars := 
+  Fixpoint modVars(s: cmd): vars := 
     match s with
-    | SLoad v _ => singleton_set v
-    | SStore _ _ => empty_set
-    | SSet v _ => singleton_set v
-    | SIf _ s1 s2 => union (modVars s1) (modVars s2)
-    | SWhile _ body => modVars body
-    | SSeq s1 s2 => union (modVars s1) (modVars s2)
-    | SSkip => empty_set
-    | SCall binds _ _ => of_list binds
+    | cmd.store _ _ _ => empty_set
+    | cmd.set v _ => singleton_set v
+    | cmd.cond _ s1 s2 => union (modVars s1) (modVars s2)
+    | cmd.while _ body => modVars body
+    | cmd.seq s1 s2 => union (modVars s1) (modVars s2)
+    | cmd.skip => empty_set
+    | cmd.call binds _ _ => of_list binds
+    | cmd.interact binds _ _ => of_list binds
     end.
 
   Lemma modVars_subset_allVars: forall x s,
     x \in modVars s ->
-    In x (allVars_stmt s).
+    In x (allVars_cmd s).
   Proof.
     intros.
     induction s; simpl in *.
     - set_solver.
     - set_solver.
-    - apply singleton_set_spec in H. auto.
+    - exfalso. eapply empty_set_spec. eassumption.
     - apply union_spec in H.
       apply in_or_app. right. apply in_or_app.
       destruct H as [H|H]; auto.
-    - apply in_or_app. right. auto.
     - apply union_spec in H.
       apply in_or_app.
       destruct H as [H|H]; auto.
-    - eapply empty_set_spec. eassumption.
+    - apply in_or_app. right. auto.
     - generalize dependent binds; induction binds; intros H; cbn in *.
       + apply empty_set_spec in H; destruct H.
       + apply union_spec in H; destruct H.
         * left. apply singleton_set_spec in H. auto.
         * right. auto.
+    - replace actname with Empty_set in *. destruct action.
   Qed.
 
 End ExprImp1.
 
 
-Ltac invert_eval_stmt :=
+Ltac invert_eval_cmd :=
   lazymatch goal with
-  | E: eval_stmt _ (S ?fuel) _ _ ?s = Some _ |- _ =>
+  | E: eval_cmd _ (S ?fuel) _ _ ?s = Some _ |- _ =>
     destruct s;
-    [ apply invert_eval_SLoad in E
-    | apply invert_eval_SStore in E
-    | apply invert_eval_SSet in E
-    | apply invert_eval_SIf in E
-    | apply invert_eval_SWhile in E
-    | apply invert_eval_SSeq in E
-    | apply invert_eval_SSkip in E
-    | apply invert_eval_SCall in E
-    ];
+    [ apply invert_eval_skip in E
+    | apply invert_eval_set in E
+    | apply invert_eval_store in E
+    | apply invert_eval_cond in E
+    | apply invert_eval_seq in E
+    | apply invert_eval_while in E
+    | apply invert_eval_call in E
+    | apply invert_eval_interact in E ];
     deep_destruct E;
-    [ let x := fresh "Case_SLoad" in pose proof tt as x; move x at top
-    | let x := fresh "Case_SStore" in pose proof tt as x; move x at top
-    | let x := fresh "Case_SSet" in pose proof tt as x; move x at top
-    | let x := fresh "Case_SIf_Then" in pose proof tt as x; move x at top
-    | let x := fresh "Case_SIf_Else" in pose proof tt as x; move x at top
-    | let x := fresh "Case_SWhile_Done" in pose proof tt as x; move x at top
-    | let x := fresh "Case_SWhile_NotDone" in pose proof tt as x; move x at top
-    | let x := fresh "Case_SSeq" in pose proof tt as x; move x at top
-    | let x := fresh "Case_SSkip" in pose proof tt as x; move x at top 
-    | let x := fresh "Case_SCall" in pose proof tt as x; move x at top
+    [ let x := fresh "Case_skip" in pose proof tt as x; move x at top 
+    | let x := fresh "Case_set" in pose proof tt as x; move x at top
+    | let x := fresh "Case_store" in pose proof tt as x; move x at top
+    | let x := fresh "Case_cond_Then" in pose proof tt as x; move x at top
+    | let x := fresh "Case_cond_Else" in pose proof tt as x; move x at top
+    | let x := fresh "Case_seq" in pose proof tt as x; move x at top
+    | let x := fresh "Case_while_Done" in pose proof tt as x; move x at top
+    | let x := fresh "Case_while_NotDone" in pose proof tt as x; move x at top
+    | let x := fresh "Case_call" in pose proof tt as x; move x at top
+    | let x := fresh "Case_interact" in pose proof tt as x; move x at top
     ]
   end.
 
 
 Section ExprImp2.
 
-  Context {mword: Set}.
-  Context {MW: MachineWidth mword}.
+  Context {p : unique! Semantics.parameters}.
 
-  Context {Name: NameWithEq}.
-  Notation var := (@name Name).
-  Existing Instance eq_name_dec.
-  Context {FName: NameWithEq}.
-  Notation func := (@name FName).
+  Notation mword := (@Semantics.word p).
+  Context {MW: MachineWidth mword}.  
+  
+  Notation var := (@varname (@syntax p)).
+  Notation func := (@funname (@syntax p)).
 
-  Context {stateMap: MapFunctions var mword}.
+  Context {stateMap: MapFunctions var (mword)}.
   Notation state := (map var mword).
   Context {varset: SetFunctions var}.
   Notation vars := (set var).
 
-  Context {funcMap: MapFunctions func (list var * list var * @stmt Name FName)}.
-  Notation env := (map func (list var * list var * stmt)).
+  (* TODO this one should be wrapped somewhere *)
+  Context {varname_eq_dec: DecidableEq var}.
+  
+  Hypothesis actname_empty: actname = Empty_set.
+  
+  Ltac state_calc := state_calc_generic (@varname (@syntax p)) (@Semantics.word p).
+  Ltac set_solver := set_solver_generic (@varname (@syntax p)).
 
-  Ltac state_calc := state_calc_generic (@name Name) mword.
+  Context {funcMap: MapFunctions func (list var * list var * @cmd (@syntax p))}.
+  Notation env := (map func (list var * list var * cmd)).
 
   Lemma modVarsSound: forall (e: env) fuel s initialS initialM finalS finalM,
-    eval_stmt e fuel initialS initialM s = Some (finalS, finalM) ->
+    eval_cmd e fuel initialS initialM s = Some (finalS, finalM) ->
     only_differ initialS (modVars s) finalS.
   Proof.
     induction fuel; introv Ev.
     - discriminate.
-    - invert_eval_stmt; simpl in *; inversionss;
+    - invert_eval_cmd; simpl in *; inversionss;
       repeat match goal with
       | IH: _, H: _ |- _ =>
           let IH' := fresh IH in pose proof IH as IH';
