compiler/src/NamesInstance.v
@@ -1,0 +1,10 @@
+Require Import Coq.ZArith.BinInt.
+Require Import bedrock2.Syntax.
+Require Import compiler.Op.
+
+Instance Names: bedrock2.Syntax.parameters := {|
+  bedrock2.Syntax.varname := Z;
+  bedrock2.Syntax.funname := Z;
+  bedrock2.Syntax.actname := Empty_set;
+  bedrock2.Syntax.bopname := binop;
+|}.
